theories/machine_base.v
@@ -49,11 +49,13 @@ Inductive instr: Type :=
 | Lea (dst: RegName) (r: Z + RegName)
 | Restrict (dst: RegName) (r: Z + RegName)
 | Subseg (dst: RegName) (r1 r2: Z + RegName)
-| IsPtr (dst r: RegName)
-| GetP (dst r: RegName)
 | GetB (dst r: RegName)
 | GetE (dst r: RegName)
 | GetA (dst r: RegName)
+| GetP (dst r: RegName) (* corresponds to CGetPerm in CHERI MIPS *)
+| GetTag (dst r: RegName) (* previously IsPtr, corresponds to CGetTag in CHERI MIPS *)
+(* | GetSealed (dst r: RegName) (* corresponds to CGetSealed in CHERI MIPS *) *)
+(* | GetOType (dst r: RegName) (* corresponds to CGetType in CHERI MIPS *) *)
 | Seal (dst : RegName) (r1 r2: RegName)
 | UnSeal (dst : RegName) (r1 r2: RegName)
 | Fail
@@ -719,7 +721,7 @@ Proof.
       | Lea dst r => GenNode 8 [GenLeaf (inl dst); GenLeaf (inr r)]
       | Restrict dst r => GenNode 9 [GenLeaf (inl dst); GenLeaf (inr r)]
       | Subseg dst r1 r2 => GenNode 10 [GenLeaf (inl dst); GenLeaf (inr r1); GenLeaf (inr r2)]
-      | IsPtr dst r => GenNode 11 [GenLeaf (inl dst); GenLeaf (inl r)]
+      | GetTag dst r => GenNode 11 [GenLeaf (inl dst); GenLeaf (inl r)]
       | GetP dst r => GenNode 13 [GenLeaf (inl dst); GenLeaf (inl r)]
       | GetB dst r => GenNode 14 [GenLeaf (inl dst); GenLeaf (inl r)]
       | GetE dst r => GenNode 15 [GenLeaf (inl dst); GenLeaf (inl r)]
@@ -742,7 +744,7 @@ Proof.
       | GenNode 8 [GenLeaf (inl dst); GenLeaf (inr r)] => Lea dst r
       | GenNode 9 [GenLeaf (inl dst); GenLeaf (inr r)] => Restrict dst r
       | GenNode 10 [GenLeaf (inl dst); GenLeaf (inr r1); GenLeaf (inr r2)] => Subseg dst r1 r2
-      | GenNode 11 [GenLeaf (inl dst); GenLeaf (inl r)] => IsPtr dst r
+      | GenNode 11 [GenLeaf (inl dst); GenLeaf (inl r)] => GetTag dst r
       | GenNode 13 [GenLeaf (inl dst); GenLeaf (inl r)] => GetP dst r
       | GenNode 14 [GenLeaf (inl dst); GenLeaf (inl r)] => GetB dst r
       | GenNode 15 [GenLeaf (inl dst); GenLeaf (inl r)] => GetE dst r
