theories/ftlr_binary/GetTag_binary.v
@@ -3,7 +3,7 @@ From iris.proofmode Require Import proofmode.
 From iris.program_logic Require Import weakestpre adequacy lifting.
 From stdpp Require Import base.
 From cap_machine Require Import ftlr_base_binary.
-From cap_machine.rules_binary Require Import rules_binary_base rules_binary_IsPtr.
+From cap_machine.rules_binary Require Import rules_binary_base rules_binary_GetTag.
 
 Section fundamental.
   Context {Σ:gFunctors} {memg:memG Σ} {regg:regG Σ}
@@ -16,25 +16,25 @@ Section fundamental.
   Implicit Types w : (leibnizO Word).
   Implicit Types interp : (D).
 
-  Lemma IsPtr_spec_determ r dst src regs regs' retv retv' :
-    IsPtr_spec r dst src regs retv ->
-    IsPtr_spec r dst src regs' retv' ->
+  Lemma GetTag_spec_determ r dst src regs regs' retv retv' :
+    GetTag_spec r dst src regs retv ->
+    GetTag_spec r dst src regs' retv' ->
     (regs = regs' ∨ retv = FailedV) ∧ retv = retv'.
   Proof.
     intros Hspec1 Hspec2.
     inversion Hspec1; inversion Hspec2; subst; simplify_eq; split; auto.
   Qed.
 
-  Lemma isptr_case (r : prodO (leibnizO Reg) (leibnizO Reg)) (p : Perm)
+  Lemma get_tag_case (r : prodO (leibnizO Reg) (leibnizO Reg)) (p : Perm)
         (b e a : Addr) (w w' : Word) (dst : RegName) (src : RegName) (P : D):
-    ftlr_instr r p b e a w w' (IsPtr dst src) P.
+    ftlr_instr r p b e a w w' (GetTag dst src) P.
   Proof.
     intros Hp Hsome HisCorrect Hbae Hi.
     iIntros "#IH #Hspec #Hinv #Hreg #Hinva #Hread Hsmap Hown Hs Ha Ha' HP Hcls HPC Hmap".
     rewrite delete_insert_delete.
     iDestruct ((big_sepM_delete _ _ PC) with "[HPC Hmap]") as "Hmap /=";
       [apply lookup_insert|rewrite delete_insert_delete;iFrame|]. simpl.
-    iApply (wp_IsPtr with "[$Ha $Hmap]"); eauto.
+    iApply (wp_GetTag with "[$Ha $Hmap]"); eauto.
     { simplify_map_eq. reflexivity. }
     { rewrite /subseteq /map_subseteq /set_subseteq_instance. intros rr _.
       apply elem_of_dom. apply lookup_insert_is_Some'; eauto. destruct Hsome with rr; eauto. }
@@ -46,7 +46,7 @@ Section fundamental.
     destruct r as [r1 r2]. simpl in *.
     iDestruct (interp_reg_eq r1 r2 (WCap p b e a) with "[]") as %Heq;[iSplit;auto|]. rewrite -!Heq.
 
-    iMod (step_IsPtr _ [SeqCtx] with "[$Ha' $Hsmap $Hs $Hspec]") as (retv' regs'') "(Hs' & Hs & Ha' & Hsmap) /=";[rewrite Heqw in Hi|..];eauto.
+    iMod (step_GetTag _ [SeqCtx] with "[$Ha' $Hsmap $Hs $Hspec]") as (retv' regs'') "(Hs' & Hs & Ha' & Hsmap) /=";[rewrite Heqw in Hi|..];eauto.
     { rewrite lookup_insert. eauto. }
     { rewrite /subseteq /map_subseteq /set_subseteq_instance. intros rr _.
       apply elem_of_dom. destruct (decide (PC = rr));[subst;rewrite lookup_insert;eauto|rewrite lookup_insert_ne //].
@@ -54,7 +54,7 @@ Section fundamental.
     { solve_ndisj. }
     iDestruct "Hs" as %HSpec'.
 
-    specialize (IsPtr_spec_determ _ _ _ _ _ _ _ HSpec HSpec') as [Hregs <-].
+    specialize (GetTag_spec_determ _ _ _ _ _ _ _ HSpec HSpec') as [Hregs <-].
 
     destruct HSpec; cycle 1.
     { iApply wp_pure_step_later; auto.
