theories/fundamental.v
@@ -1,4 +1,4 @@
-From cap_machine.ftlr Require Export Jmp Jnz Mov Load Store AddSubLt Restrict Subseg IsPtr Get Lea Seal UnSeal.
+From cap_machine.ftlr Require Export Jmp Jnz Mov Load Store AddSubLt Restrict Subseg GetTag Get Lea Seal UnSeal.
 From iris.proofmode Require Import proofmode.
 From iris.program_logic Require Import weakestpre adequacy lifting.
 From stdpp Require Import base.
@@ -92,12 +92,6 @@ Section fundamental.
       + (* Subseg *)
         iApply (subseg_case with "[] [] [] [] [] [Hown] [Ha] [HP] [Hcls] [HPC] [Hmap]");
           try iAssumption; eauto.
-      + (* IsPtr *)
-        iApply (isptr_case with "[] [] [] [] [] [Hown] [Ha] [HP] [Hcls] [HPC] [Hmap]");
-          try iAssumption; eauto.
-      + (* GetP *)
-        iApply (get_case _ _ _ _ _ _ _ _ (GetP _ _) with "[] [] [] [] [] [Hown] [Ha] [HP] [Hcls] [HPC] [Hmap]");
-          try iAssumption; eauto.
       + (* GetB *)
         iApply (get_case _ _ _ _ _ _ _ _ (GetB _ _) with "[] [] [] [] [] [Hown] [Ha] [HP] [Hcls] [HPC] [Hmap]");
           try iAssumption; eauto.
@@ -106,6 +100,12 @@ Section fundamental.
           try iAssumption; eauto.
       + (* GetA *)
         iApply (get_case _ _ _ _ _ _ _ _ (GetA _ _) with "[] [] [] [] [] [Hown] [Ha] [HP] [Hcls] [HPC] [Hmap]");
+          try iAssumption; eauto.
+      + (* GetP *)
+        iApply (get_case _ _ _ _ _ _ _ _ (GetP _ _) with "[] [] [] [] [] [Hown] [Ha] [HP] [Hcls] [HPC] [Hmap]");
+          try iAssumption; eauto.
+      + (* GetTag *)
+        iApply (get_tag_case with "[] [] [] [] [] [Hown] [Ha] [HP] [Hcls] [HPC] [Hmap]");
           try iAssumption; eauto.
       + (* Seal *)
         iApply (seal_case with "[] [] [] [] [] [Hown] [Ha] [HP] [Hcls] [HPC] [Hmap]");
