theories/rules/rules_Mov.v
@@ -18,7 +18,7 @@ Section cap_lang_rules.
   Implicit Types ms : gmap Addr Word.
 
   Inductive Mov_spec (regs: Reg) (dst: RegName) (src: Z + RegName) (regs': Reg): cap_lang.val -> Prop :=
-  | IsPtr_spec_success w:
+  | GetTag_spec_success w:
       word_of_argument regs src = Some w →
       incrementPC (<[ dst := w ]> regs) = Some regs' →
       Mov_spec regs dst src regs' NextIV
